Refactor state

theories/Commons/Behaviors.v
@@ -1,11 +1,14 @@
 From RSL Require Import Prelude.
 
+From RSL.Commons Require Import Language.
+
 From Stdlib Require Import Classical.
+
 From Coinduction Require Import all.
 
 Section Behavior.
   Context {Λ: lang} (P: prog Λ).
-  Implicit Type s : state Λ.
+  Implicit Types s : state Λ.
 
   Program Definition diverges_: mon (state Λ -> Prop) :=
     {| body R s := ∃ s', P ⊨ s ->> s' ∧ R s' |}.
@@ -43,15 +46,15 @@ Section Behavior.
   Qed.
 
   Variant behavior :=
-  | Terminating (v: value Λ)
+  | Terminating (v: value Λ) (m: memory)
   | Diverging
   | Undef.
 
   (* [beh s] is the set of all the behaviors of [s] *)
   Inductive beh : behavior -> state Λ -> Prop :=
-  | IsTerminating : ∀ s v,
-      is_final s = Some v ->
-      beh (Terminating v) s
+  | IsTerminating : ∀ s v m,
+      is_final s = Some (v, m) ->
+      beh (Terminating v m) s
   | IsDiverging : ∀ s,
       diverges s ->
       beh Diverging s
@@ -66,17 +69,17 @@ Section Behavior.
   Global Instance beh_elem_state : ElemOf behavior (state Λ) := beh.
 
   (* [s] is terminating iff there is a execution from [s] to a final state. *)
-  Lemma has_terminating_behavior : ∀ s v,
-    Terminating v ∈ s <-> ∃ t, P ⊨ s ->>* t ∧ is_final t = Some v.
+  Lemma has_terminating_behavior : ∀ s v m,
+    Terminating v m ∈ s <-> ∃ s', P ⊨ s ->>* s' ∧ is_final s' = Some (v, m).
   Proof using Type.
-    intros s v. split; intros Hbeh.
-    - remember (Terminating v) as b eqn:Hb.
+    intros s v m. split; intros Hbeh.
+    - remember (Terminating v m) as b eqn:Hb.
       induction Hbeh as [ s | | | s t b ? IH Hstep ]; inv Hb; auto.
       + exists s. now constructor.
-      + destruct (IH eq_refl) as (t' & Hrtc & Hfin). clear IH.
-        exists t'. split; eauto. now apply rtc_l with t.
-    - destruct Hbeh as (t & Hrtc & Hfin).
-      induction Hrtc as [ | s t u Hstep Hrtc IH ].
+      + destruct (IH eq_refl) as (s' & Hrtc & Hfin). clear IH.
+        exists s'. split; eauto. now apply rtc_l with t.
+    - destruct Hbeh as (s' & Hrtc & Hfin).
+      induction Hrtc as [ | s ? u Hstep Hrtc IH ].
       + now constructor.
       + eapply IsSteping; eauto. now apply IH.
   Qed.
@@ -108,7 +111,7 @@ Section Behavior.
         * now apply rtc_l with t.
         * assumption.
     - destruct Hbeh as (u & Hrtc & Hstuck).
-      induction Hrtc  as [ | s t u Hstep Hrtc IH].
+      induction Hrtc  as [ | s t ? Hstep Hrtc IH].
       + now constructor.
       + eapply IsSteping.
         * now apply IH.
@@ -116,7 +119,7 @@ Section Behavior.
   Qed.
 
   Definition does_end s : Prop :=
-    ∃ t, P ⊨ s ->>* t ∧ ((∃ v, is_final t = Some v) ∨ stuck P t).
+    ∃ t, P ⊨ s ->>* t ∧ (is_Some (is_final t) ∨ stuck P t).
 
   Lemma not_ending_diverges:
     ∀ s, ~(does_end s) -> ∀ t, P ⊨ s ->>* t -> diverges t.
@@ -128,23 +131,25 @@ Section Behavior.
       intros t Hstep. apply not_ex_all_not with (n := t) in H.
       split.
       - destruct (is_final t) as [v | ].
-        + exfalso. apply H. split; auto. left. now eexists.
+        + exfalso. apply H. split; auto.
         + reflexivity.
       - intro Hs. apply H. now auto.
     }
     intros t Hrtc.
     destruct (Hs t) as [Hnfin Hnstuck]; auto.
     unfold stuck in Hnstuck.
-    assert (Hprogress: can_progress P t) by tauto.
-    destruct (can_progress_must_step _ _ Hprogress) as [u Hstep].
-    exists u. split; auto.
-    apply cih. eapply rtc_r; eassumption.
+    destruct (classic (can_progress P t)) as [Hprog | HnProg].
+    - destruct (can_progress_must_step _ _ Hprog) as [u Hstep].
+      exists u. split; auto.
+      apply cih. eapply rtc_r; eassumption.
+    - exfalso. apply Hnstuck. split; auto.
   Qed.
 
   Theorem every_state_has_beh : ∀ s, ∃ b, b ∈ s.
   Proof using Type.
-    intros s. destruct (classic (does_end s)) as [(t & Hrtc & [[v Hfin] | H]) | H].
-    - exists (Terminating v). apply has_terminating_behavior.
+    intros s. destruct (classic (does_end s)) as [(t & Hrtc & [Hfin | H]) | H].
+    - destruct Hfin as [[v m] Hfin].
+      exists (Terminating v m). apply has_terminating_behavior.
       exists t; auto.
     - exists Undef. apply has_undef_behavior.
       exists t; auto.
@@ -160,11 +165,13 @@ Section Refinement.
   Instance behₜ_elem : ElemOf behavior (state Λₜ) := beh Pₜ.
   Instance behₛ_elem : ElemOf behavior (state Λₛ) := beh Pₛ.
 
-  Inductive behavior_order Φ : @behavior Λₜ -> @behavior Λₛ -> Prop :=
-  | TerminatingOrder : ∀ (vₜ: value Λₜ) (vₛ: value Λₛ),
-    Φ vₜ vₛ -> behavior_order Φ (Terminating vₜ) (Terminating vₛ)
-  | DivergingOrder : behavior_order Φ Diverging Diverging
-  | UndefOrder : ∀ s, behavior_order Φ s Undef.
+  Variant behavior_order Φ : @behavior Λₜ -> @behavior Λₛ -> Prop :=
+  | BehOrderTerm vt vs mt ms :
+      Φ (vt, mt) (vs, ms) -> behavior_order Φ (Terminating vt mt) (Terminating vs ms)
+  | BehOrderDiv :
+      behavior_order Φ Diverging Diverging
+  | BehOrderUndef bt :
+      behavior_order Φ bt Undef.
 
   Notation "a '⊑{' Φ '}' b" :=
     (behavior_order Φ a b)
@@ -176,6 +183,7 @@ Section Refinement.
   (*    - if the target diverges, *)
   (*    the source must either diverges or be stuck. *)
   (*    - if the target is stuck, the source should also be stuck. *)
-  Definition refines Φ (t: state Λₜ) (s: state Λₛ) :=
+  Definition refines Φ (t: state Λₜ) (s: state Λₛ) : Prop :=
     ∀ b, b ∈ t -> ∃ b', b' ∈ s ∧ b ⊑{Φ} b'.
+
 End Refinement.
