theories/Logic.v
@@ -1,0 +1,2 @@
+From RSL Require Export Logic.Logic.
+From RSL Require Export Logic.Memory.
