theories/RelLogic.v
@@ -1,2 +1,0 @@
-From RSL Require Export RelLogic.Logic.
-From RSL Require Export RelLogic.Memory.
