theories/Simulations/FreeSimRules.v
@@ -16,11 +16,11 @@ Section FSimRules.
   Implicit Types (C: Chain fsim_lfp).
 
   Lemma fsim_in_chain Post:
-    ∀ j t i s,
-    (∀ C, fsim_lfp (elem C) Post j t i s) ->
-    fsim Post j t i s.
+    ∀ t j i s,
+    (∀ C, fsim_lfp (elem C) Post t j i s) ->
+    fsim Post t j i s.
   Proof using Type.
-    intros j t i s Hr.
+    intros t j i s Hr.
     unfold fsim.
     apply (gfp_prop).
     intros C.
@@ -28,73 +28,73 @@ Section FSimRules.
   Qed.
 
   Lemma final C Post:
-    ∀ j t i s,
+    ∀ t j i s,
     both_final Post t s ->
-    elem C Post j t i s.
+    elem C Post t j i s.
   Proof using Type.
     apply tower.
-    { intros P Hp j t i s H Q Hq. eapply Hp; now eauto. }
-    intros C' CIH j t i s H. econstructor; now eauto.
+    { intros P Hp t j i s H Q Hq. eapply Hp; now eauto. }
+    intros C' CIH t j i s H. econstructor; now eauto.
   Qed.
 
   Lemma stuck C Post:
-    ∀ j t i s,
+    ∀ t j i s,
     stuck Pₛ s ->
-    elem C Post j t i s.
+    elem C Post t j i s.
   Proof using Type.
     apply tower.
-    { intros P Hp j t i s H Q Hq. eapply Hp; now eauto. }
-    intros C' CIH j t i s H. econstructor; now eauto.
+    { intros P Hp t j i s H Q Hq. eapply Hp; now eauto. }
+    intros C' CIH t j i s H. econstructor; now eauto.
   Qed.
 
   Lemma source_step C Post:
     ∀ j t i i' s s',
     Pₛ ⊨ s ->> s' ->
-    elem C Post j t i' s' ->
-    elem C Post j t i s.
+    elem C Post t j i' s' ->
+    elem C Post t j i s.
   Proof using Type.
     apply tower.
-    { intros P Hp j t i i' s s' Hstep H Q Hq. eapply Hp; now eauto. }
-    intros C' CIH j t i i' s s' Hstep H. econstructor; now eauto.
+    { intros P Hp t j i i' s s' Hstep H Q Hq. eapply Hp; now eauto. }
+    intros C' CIH t j i i' s s' Hstep H. econstructor; now eauto.
   Qed.
 
   Lemma target_step C Post:
-    ∀ j t i s,
+    ∀ t j i s,
     can_progress Pₜ t ->
-    (∀ t', Pₜ ⊨ t ->> t' -> ∃ j', elem C Post j' t' i s) ->
-    elem C Post j t i s.
+    (∀ t', Pₜ ⊨ t ->> t' -> ∃ j', elem C Post t' j' i s) ->
+    elem C Post t j i s.
   Proof using Type.
     apply tower.
-    { intros P Hp j t i s Hprogesss H Q Hq.
+    { intros P Hp t j i s Hprogesss H Q Hq.
       eapply Hp; eauto.
       intros t' Hstep. destruct (H _ Hstep) as [j' Hinf].
       exists j'. now auto. }
-    intros C' CIH j t i s Hprogress Ht. econstructor; now eauto.
+    intros C' CIH t j i s Hprogress Ht. econstructor; now eauto.
   Qed.
 
   Lemma progress_step C Post:
-    ∀ j j' t i i' s,
+    ∀ t j j' i i' s,
     j' ⊏ j ->
     i' ⊏ i ->
-    elem C Post j' t i' s ->
-    elem C Post j t i s.
+    elem C Post t j' i' s ->
+    elem C Post t j i s.
   Proof using Type.
     apply tower.
-    { intros P Hp j j' t i i' s Ht Hs H Q Hq.
+    { intros P Hp t j j' i i' s Ht Hs H Q Hq.
       eapply Hp; now eauto. }
-    intros C' CIH j j' t i i' s Ht Hs H.
+    intros C' CIH t j j' i i' s Ht Hs H.
     eapply FProgress; try eassumption.
     now apply (b_chain C').
   Qed.
 
   Lemma coind_weak C Post:
-    ∀ j t i s,
+    ∀ t j i s,
     (∀ C,
-       (∀ j' i', j ⊏ j' -> i ⊏ i' -> fsim_lfp (elem C) Post j' t i' s) ->
-       fsim_lfp (elem C) Post j t i s) ->
-    elem C Post j t i s.
+       (∀ j' i', j ⊏ j' -> i ⊏ i' -> fsim_lfp (elem C) Post t j' i' s) ->
+       fsim_lfp (elem C) Post t j i s) ->
+    elem C Post t j i s.
   Proof using Type.
-    intros j t i s RIH.
+    intros t j i s RIH.
     apply tower.
     { intros P Hp Q Hq. eapply Hp; now eauto. }
     intros C' CIH.
@@ -102,64 +102,64 @@ Section FSimRules.
     eapply FProgress; now eauto.
   Qed.
 
-  Lemma coind_strong C Post P:
-    (∀ C j t i s,
+  Lemma coind_strong C Post (Inv: _ -> state Λₜ -> J -> I -> state Λₛ -> Prop) :
+    (∀ C t j i s,
        (∀ j' t i' s,
-          P Post j t i s ->
+          Inv Post t j i s ->
           j ⊏ j' ->
           i ⊏ i' ->
-          fsim_lfp (elem C) Post j' t i' s) ->
-       P Post j t i s ->
-       fsim_lfp (elem C) Post j t i s) ->
-    ∀ j t i s,
-    P Post j t i s ->
-    elem C Post j t i s.
+          fsim_lfp (elem C) Post t j' i' s) ->
+       Inv Post t j i s ->
+       fsim_lfp (elem C) Post t j i s) ->
+    ∀ t j i s,
+    Inv Post t j i s ->
+    elem C Post t j i s.
   Proof using Type.
     intros RIH.
     apply tower.
-    { intros Z Hz j t i s HP Q Hq. eapply Hz; now eauto. }
-    intros C' CIH j t i s HP.
+    { intros Z Hz t j i s HP Q Hq. eapply Hz; now eauto. }
+    intros C' CIH t j i s HP.
     apply RIH.
-    - intros j' t' i' s' HP' Hj Hi.
+    - intros t' j' i' s' HP' Hj Hi.
       eapply FProgress; now eauto.
     - assumption.
   Qed.
 
   Lemma coind_weak_open Post:
-    ∀ j t i s,
+    ∀ t j i s,
     (∀ R,
        (∀ j' i',
           j ⊏ j' ->
           i ⊏ i' ->
-          fsim_lfp R Post j' t i' s) ->
-       fsim_lfp R Post j t i s) ->
-    fsim_lfp fsim Post j t i s.
+          fsim_lfp R Post t j' i' s) ->
+       fsim_lfp R Post t j i s) ->
+    fsim_lfp fsim Post t j i s.
   Proof using Type.
-    intros j t i s RIH.
+    intros t j i s RIH.
     apply fsim_unroll.
     coinduction C CIH.
     apply RIH. intros j' i' Hj Hi.
     eapply FProgress; now eauto.
   Qed.
 
-  Lemma coind_strong_open Post P:
-    (∀ R j t i s,
+  Lemma coind_strong_open Post (Inv: _ -> state Λₜ -> J -> I -> state Λₛ -> Prop) :
+    (∀ R t j i s,
        (∀ j' t i' s,
-          P Post j t i s ->
+          Inv Post t j i s ->
           j ⊏ j' ->
           i ⊏ i' ->
-          fsim_lfp R Post j' t i' s) ->
-       P Post j t i s ->
-       fsim_lfp R Post j t i s) ->
-    ∀ j t i s,
-    P Post j t i s ->
-    fsim_lfp fsim Post j t i s.
+          fsim_lfp R Post t j' i' s) ->
+       Inv Post t j i s ->
+       fsim_lfp R Post t j i s) ->
+    ∀ t j i s,
+    Inv Post t j i s ->
+    fsim_lfp fsim Post t j i s.
   Proof using Type.
-    intros RIH j t i s HP.
+    intros RIH t j i s HP.
     apply fsim_unroll.
-    revert j t i s HP.
+    revert t j i s HP.
     coinduction C CIH.
-    intros j t i s HP.
+    intros t j i s HP.
     apply RIH.
     - intros j' t' i' s' Hj Hi HP'.
       eapply FProgress; now eauto.
